lemmas about function and permutation versions of MatchSubst

src/FcEtt/ett_match.v
@@ -11,6 +11,326 @@ Require Export FcEtt.ett_ind.
 Require Export FcEtt.toplevel.
 Require Export FcEtt.fix_typing.
 
+Require Import Coq.Sorting.Permutation.
+
+Fixpoint matchsubst a p b : tm := match (a,p) with
+  | (a_Fam F, a_Fam F') => b
+  | (a_App a1 (Role Nom) a2, a_App p1 (Role Nom) (a_Var_f x)) =>
+         tm_subst_tm_tm a2 x (matchsubst a1 p1 b)
+  | (a_App a1 (Role Rep) a2, a_App p1 (Role Rep) (a_Var_f x)) =>
+         tm_subst_tm_tm a2 x (matchsubst a1 p1 b)
+  | (a_App a1 (Rho Irrel) a_Bullet, a_App p1 (Rho Irrel) a_Bullet) =>
+         matchsubst a1 p1 b
+  | (a_CApp a1 g_Triv, a_CApp p1 g_Triv) => matchsubst a1 p1 b
+  | (_,_) => b
+  end.
+
+Lemma MatchSubst_matchsubst : forall a p b b',
+      MatchSubst a p b b' -> matchsubst a p b = b'.
+Proof. intros. induction H.
+        - simpl. auto.
+        - destruct R; simpl. rewrite IHMatchSubst. auto.
+          rewrite IHMatchSubst. auto.
+        - simpl. auto.
+        - simpl. auto.
+Qed.
+
+Corollary MatchSubst_function : forall a p b b1 b2,
+      MatchSubst a p b b1 -> MatchSubst a p b b2 -> b1 = b2.
+Proof. intros. apply MatchSubst_matchsubst in H.
+       apply MatchSubst_matchsubst in H0. rewrite H in H0. auto.
+Qed.
+
+Inductive Path_pat_consist : tm -> tm -> Prop :=
+  | Path_consist_Fam : forall F, Path_pat_consist (a_Fam F) (a_Fam F)
+  | Path_consist_AppR : forall a1 p1 a2 x R, Path_pat_consist a1 p1 -> lc_tm a2 ->
+       Path_pat_consist (a_App a1 (Role R) a2) (a_App p1 (Role R) (a_Var_f x))
+  | Path_consist_IApp : forall a1 p1, Path_pat_consist a1 p1 ->
+       Path_pat_consist (a_App a1 (Rho Irrel) a_Bullet)
+                        (a_App p1 (Rho Irrel) a_Bullet)
+  | Path_consist_CApp : forall a1 p1, Path_pat_consist a1 p1 ->
+       Path_pat_consist (a_CApp a1 g_Triv) (a_CApp p1 g_Triv).
+
+Hint Constructors Path_pat_consist.
+
+Lemma MatchSubst_consist : forall a p b b', MatchSubst a p b b' ->
+                                            Path_pat_consist a p.
+Proof. intros. induction H; eauto.
+Qed.
+
+Corollary MatchSubst_nexists : forall a p, ~(Path_pat_consist a p) ->
+                      forall b b', ~(MatchSubst a p b b').
+Proof. intros. intro H'. apply MatchSubst_consist in H'. contradiction.
+Qed.
+
+Lemma MatchSubst_exists : forall a p, Path_pat_consist a p -> forall b,
+                          lc_tm b -> exists b', MatchSubst a p b b'.
+Proof. intros a p H. induction H; intros.
+        - exists b; auto.
+        - pose (P := IHPath_pat_consist b H1). inversion P as [b1 Q].
+          exists (tm_subst_tm_tm a2 x b1). eauto.
+        - pose (P := IHPath_pat_consist b H0). inversion P as [b1 Q].
+          exists b1; eauto.
+        - pose (P := IHPath_pat_consist b H0). inversion P as [b1 Q].
+          exists b1; eauto.
+Qed.
+
+Lemma matchsubst_MatchSubst : forall a p b b', Path_pat_consist a p -> lc_tm b ->
+      matchsubst a p b = b' -> MatchSubst a p b b'.
+Proof. intros. generalize dependent b. generalize dependent b'.
+       induction H; intros; eauto.
+        - simpl in H1. rewrite <- H1. auto.
+        - destruct R. simpl in H2. rewrite <- H2. eauto.
+          simpl in H2. rewrite <- H2. eauto.
+Qed.
+
+Inductive Pattern : tm -> Prop :=
+  | Pattern_Fam : forall F, Pattern (a_Fam F)
+  | Pattern_AppR : forall a1 R x, Pattern a1 -> Pattern (a_App a1 (Role R) (a_Var_f x))
+  | Pattern_IApp : forall a1, Pattern a1 -> Pattern (a_App a1 (Rho Irrel) a_Bullet)
+  | Pattern_CApp : forall a1, Pattern a1 -> Pattern (a_CApp a1 g_Triv).
+
+Hint Constructors Pattern.
+
+Lemma Path_pat_consist_pat : forall a p, Path_pat_consist a p -> Pattern p.
+Proof. intros. induction H; eauto.
+Qed.
+
+Fixpoint chain_substitution (l : list (atom * tm)) (b : tm) : tm :=
+   match l with
+   | nil => b
+   | (x, a) :: l' => tm_subst_tm_tm a x (chain_substitution l' b)
+   end.
+
+Fixpoint permutation (a p : tm) : list (atom * tm) := match (a,p) with
+  | (a_Fam F, a_Fam F') => nil
+  | (a_App a1 (Role Nom) a2, a_App p1 (Role Nom) (a_Var_f x)) =>
+         (x, a2) :: permutation a1 p1
+  | (a_App a1 (Role Rep) a2, a_App p1 (Role Rep) (a_Var_f x)) =>
+         (x, a2) :: permutation a1 p1
+  | (a_App a1 (Rho Irrel) a_Bullet, a_App p1 (Rho Irrel) a_Bullet) =>
+         permutation a1 p1
+  | (a_CApp a1 g_Triv, a_CApp p1 g_Triv) => permutation a1 p1
+  | (_,_) => nil
+  end.
+
+Lemma MatchSubst_permutation : forall a p b,
+              chain_substitution (permutation a p) b = matchsubst a p b.
+Proof. intros. generalize dependent p. generalize dependent b.
+       induction a; intros; eauto.
+       all: try destruct g; try destruct nu; eauto.
+       all: try destruct R; try destruct rho; eauto.
+        - destruct p; eauto. destruct nu; eauto. destruct R; eauto.
+          destruct p2; eauto. simpl. rewrite IHa1. auto.
+        - destruct p; eauto. destruct nu; eauto. destruct R; eauto.
+          destruct p2; eauto. simpl. rewrite IHa1. auto.
+        - destruct a2; eauto. destruct p; eauto. destruct nu; eauto.
+          destruct rho; eauto. destruct p2; eauto.
+        - destruct p; eauto. destruct g; eauto.
+        - destruct p; eauto.
+Qed.
+
+Inductive ICApp : tm -> tm -> Prop :=
+   | ICApp_refl : forall a, ICApp a a
+   | ICApp_IApp : forall a1 a2, ICApp a1 a2 -> ICApp a1 (a_App a2 (Rho Irrel) a_Bullet)
+   | ICApp_CApp : forall a1 a2, ICApp a1 a2 -> ICApp a1 (a_CApp a2 g_Triv).
+
+Lemma nonempty_perm : forall a p x l, x :: l = permutation a p ->
+      exists a1 a2 p1 y, (ICApp (a_App a1 (Role Nom) a2) a /\ 
+              ICApp (a_App p1 (Role Nom) (a_Var_f y)) p /\ x = (y, a2)
+              /\ l = permutation a1 p1) \/
+              (ICApp (a_App a1 (Role Rep) a2) a /\ 
+              ICApp (a_App p1 (Role Rep) (a_Var_f y)) p /\ x = (y, a2)
+              /\ l = permutation a1 p1).
+Proof. intros a. induction a; intros p y l H; try (inversion H; fail).
+       destruct nu; try (inversion H; fail).
+       destruct R; try (inversion H; fail).
+       destruct p; try (inversion H; fail).
+       destruct nu; try (inversion H; fail).
+       destruct R; try (inversion H; fail).
+       destruct p2; try (inversion H; fail).
+       inversion H. exists a1, a2, p1, x. left; repeat split.
+       eapply ICApp_refl. eapply ICApp_refl.
+       destruct p; try (inversion H; fail).
+       destruct nu; try (inversion H; fail).
+       destruct R; try (inversion H; fail).
+       destruct p2; try (inversion H; fail).
+       inversion H. exists a1, a2, p1, x. right; repeat split.
+       eapply ICApp_refl. eapply ICApp_refl.
+       destruct rho; try (inversion H; fail).
+       destruct a2; try (inversion H; fail).
+       destruct p; try (inversion H; fail).
+       destruct nu; try (inversion H; fail).
+       destruct rho; try (inversion H; fail).
+       destruct p2; try (inversion H; fail).
+       simpl in H. pose (P := IHa1 p1 y l ltac:(auto)).
+       inversion P as [a2 [a3 [p2 [y0 [Q1 | Q2]]]]]. 
+       exists a2, a3, p2, y0. inversion Q1 as [S1 [S2 [S3 S4]]].
+       left; repeat split.
+       eapply ICApp_IApp; auto.
+       eapply ICApp_IApp; auto. auto. auto.
+       exists a2, a3, p2, y0. inversion Q2 as [T1 [T2 [T3 T4]]]. 
+       right; repeat split.
+       eapply ICApp_IApp; auto.
+       eapply ICApp_IApp; auto. auto. auto.
+       destruct g; try (inversion H; fail).
+       destruct p; try (inversion H; fail).
+       destruct g; try (inversion H; fail).
+       simpl in H. pose (P := IHa p y l ltac:(auto)).
+       inversion P as [a2 [a3 [p2 [y0 [Q1 | Q2]]]]]. 
+       exists a2, a3, p2, y0. inversion Q1 as [S1 [S2 [S3 S4]]].
+       left; repeat split.
+       eapply ICApp_CApp; auto.
+       eapply ICApp_CApp; auto. auto. auto.
+       exists a2, a3, p2, y0. inversion Q2 as [T1 [T2 [T3 T4]]]. 
+       right; repeat split.
+       eapply ICApp_CApp; auto.
+       eapply ICApp_CApp; auto. auto. auto.
+       destruct p; try (inversion H; fail).
+Qed.
+
+Lemma fv_ICApp : forall a1 a2 x, ICApp a1 a2 -> x `in` fv_tm_tm_tm a1 <->
+                  x `in` fv_tm_tm_tm a2.
+Proof. intros. generalize dependent x.
+       induction H; intro.
+         - split; auto.
+         - pose (P := IHICApp x). inversion P as [P1 P2].
+           split; intro; simpl in *; fsetdec.
+         - pose (P := IHICApp x). inversion P as [P1 P2].
+           split; intro; simpl in *; fsetdec.
+Qed.
+
+Lemma fv_perm_1 : forall a p l x a', l = permutation a p -> In (x,a') l ->
+                    x `in` fv_tm_tm_tm p.
+Proof. intros. generalize dependent a. generalize dependent p.
+       dependent induction l; intros. inversion H0.
+       inversion H0. subst. apply nonempty_perm in H.
+       inversion H as [a1 [a2 [p1 [y [Q1 | Q2]]]]].
+       inversion Q1 as [S1 [S2 [S3 S4]]].
+       eapply (fv_ICApp x) in S2. inversion S3; subst. simpl in S2.
+       fsetdec. inversion Q2 as [T1 [T2 [T3 T4]]].
+       eapply (fv_ICApp x) in T2. inversion T3; subst. simpl in T2.
+       fsetdec. apply nonempty_perm in H.
+       inversion H as [a1 [a2 [p1 [y [Q1 | Q2]]]]].
+       inversion Q1 as [S1 [S2 [S3 S4]]].
+       eapply (fv_ICApp x) in S2. apply S2. simpl. apply union_iff.
+       left. eapply IHl; eauto.
+       inversion Q2 as [T1 [T2 [T3 T4]]].
+       eapply (fv_ICApp x) in T2. apply T2. simpl. apply union_iff.
+       left. eapply IHl; eauto.
+Qed.
+
+Lemma fv_perm_2 : forall a p l x a', l = permutation a p -> In (x,a') l ->
+                  forall y, y `in` fv_tm_tm_tm a' -> y `in` fv_tm_tm_tm a.
+Proof. intros. generalize dependent a. generalize dependent p.
+       dependent induction l; intros. inversion H0.
+       inversion H0. subst. apply nonempty_perm in H.
+       inversion H as [a1 [a2 [p1 [z [Q1 | Q2]]]]].
+       inversion Q1 as [S1 [S2 [S3 S4]]].
+       eapply (fv_ICApp y) in S1. inversion S3; subst. simpl in S1.
+       fsetdec. inversion Q2 as [T1 [T2 [T3 T4]]].
+       eapply (fv_ICApp y) in T1. inversion T3; subst. simpl in T1.
+       fsetdec. apply nonempty_perm in H.
+       inversion H as [a1 [a2 [p1 [z [Q1 | Q2]]]]].
+       inversion Q1 as [S1 [S2 [S3 S4]]].
+       eapply (fv_ICApp y) in S1. apply S1. simpl. apply union_iff.
+       left. eapply IHl; eauto.
+       inversion Q2 as [T1 [T2 [T3 T4]]].
+       eapply (fv_ICApp y) in T1. apply T1. simpl. apply union_iff.
+       left. eapply IHl; eauto.
+Qed.
+
+Fixpoint rang (L : list (atom * tm)) : atoms :=
+   match L with
+   | nil => empty
+   | (x, a) :: l => fv_tm_tm_tm a \u rang l
+   end.
+
+Lemma dom_Perm : forall A (L : list (atom * A)) L', Permutation L L' ->
+                                                        dom L [=] dom L'.
+Proof. intros. induction H; eauto. fsetdec. destruct x; simpl. fsetdec.
+       destruct x, y. simpl. fsetdec. eapply transitivity; eauto.
+Qed.
+
+Lemma rang_Perm : forall L L', Permutation L L' -> rang L [=] rang L'.
+Proof. intros. induction H; eauto. fsetdec. destruct x; simpl. fsetdec.
+       destruct x, y. simpl. fsetdec. eapply transitivity; eauto.
+Qed.
+
+Lemma uniq_Perm : forall A (L : list (atom * A)) L', Permutation L L' ->
+                                                      uniq L -> uniq L'.
+Proof. intros. induction H; eauto. destruct x. apply uniq_cons_iff in H0.
+       inversion H0. eapply uniq_cons_3; eauto. apply dom_Perm in H. fsetdec.
+       destruct x, y. solve_uniq.
+Qed.
+
+Lemma Chain_sub_Permutation : forall b L L',
+        uniq L -> (forall x, x `in` dom L -> x `notin` rang L) ->
+        Permutation L L' -> chain_substitution L b = chain_substitution L' b.
+Proof. intros.
+       dependent induction H1; intros.
+         - auto.
+         - simpl. destruct x. erewrite IHPermutation; eauto 1.
+           solve_uniq. intros. simpl in H0. pose (P := H0 x ltac:(auto)).
+           fsetdec.
+         - destruct x, y. simpl. rewrite tm_subst_tm_tm_tm_subst_tm_tm.
+           rewrite (tm_subst_tm_tm_fresh_eq t). auto. simpl in H0.
+           pose (P := H0 a0 ltac:(auto)). fsetdec. simpl in H0.
+           pose (P := H0 a ltac:(auto)). fsetdec.
+           solve_uniq.
+         - apply transitivity with (y := chain_substitution l' b).
+           eapply IHPermutation1; eauto. eapply IHPermutation2.
+           eapply uniq_Perm; eauto. pose (P := H1_). pose (Q := H1_).
+           apply dom_Perm in P. apply rang_Perm in Q. intros.
+           pose (S := H0 x). fsetdec.
+Qed.
+
+Definition Nice a p := Path_pat_consist a p /\
+              (forall x, x `in` fv_tm_tm_tm p -> x `notin` fv_tm_tm_tm a) /\
+               uniq (permutation a p).
+
+Fixpoint matchsubst2 a p b : tm := match (a,p) with
+  | (a_Fam F, a_Fam F') => if F == F' then b else a_Bullet
+  | (a_App a1 (Role Nom) a2, a_App p1 (Role Nom) (a_Var_f x)) =>
+         tm_subst_tm_tm a2 x (matchsubst a1 p1 b)
+  | (a_App a1 (Role Rep) a2, a_App p1 (Role Rep) (a_Var_f x)) =>
+         tm_subst_tm_tm a2 x (matchsubst a1 p1 b)
+  | (a_App a1 (Rho Irrel) a_Bullet, a_App p1 (Rho Irrel) a_Bullet) =>
+         matchsubst a1 p1 b
+  | (a_CApp a1 g_Triv, a_CApp p1 g_Triv) => matchsubst a1 p1 b
+  | (_,_) => a_Bullet
+  end.
+
+Lemma matchsubst_subst : forall a p b x y, x `notin` fv_tm_tm_tm a ->
+      y `notin` fv_tm_tm_tm a -> matchsubst2 a p b =
+    matchsubst2 a (tm_subst_tm_tm (a_Var_f y) x p) (tm_subst_tm_tm (a_Var_f y) x b).
+Proof. intros. generalize dependent p. generalize dependent b.
+       induction a; intros; eauto.
+         - destruct nu; eauto. destruct R; eauto.
+           destruct p; eauto. simpl. destruct (x0 == x); auto.
+           destruct nu; eauto. destruct R; eauto. destruct p2; eauto.
+           simpl. destruct (x0 == x); auto.
+
+Fixpoint matchsubst2 a p b : tm := match (a,p) with
+  | (a_Fam F, a_Fam F') => if F == F' then b else a_Bullet
+  | (a_App a1 (Role Nom) a2, a_App p1 (Role Nom) (a_Var_f x)) =>
+         matchsubst2 a1 p1 (tm_subst_tm_tm a2 x b)
+  | (a_App a1 (Role Rep) a2, a_App p1 (Role Rep) (a_Var_f x)) =>
+         matchsubst2 a1 p1 (tm_subst_tm_tm a2 x b)
+  | (a_App a1 (Rho Irrel) a_Bullet, a_App p1 (Rho Irrel) a_Bullet) =>
+         matchsubst a1 p1 b
+  | (a_CApp a1 g_Triv, a_CApp p1 g_Triv) => matchsubst a1 p1 b
+  | (_,_) => a_Bullet
+  end.
+
+Lemma matchsubst_matchsubst2 : forall a p b,
+      (forall x, x `in` fv_tm_tm_tm a -> x `notin` fv_tm_tm_tm p) ->
+       matchsubst a p b = matchsubst2 a p b.
+Proof. intros. generalize dependent p. generalize dependent b.
+       induction a; intros; eauto. destruct p; eauto.
+       destruct p2; eauto. destruct nu; eauto.
+       destruct nu0; eauto. destruct R, R0; eauto; simpl.
+
 
 Lemma MatchSubst_lc_1 : forall a p b b', MatchSubst a p b b' →  lc_tm a.
 Proof.
